Correctness.v
@@ -11,25 +11,17 @@ Require Import SysF.
 Lemma beq_typ_correct : forall t1 t2 : typ, beq_typ t1 t2 = true -> t1 = t2.
   induction t1.
   - intros.
-    simpl in H.
-    destruct t2.
-    + apply eq_sym in H.
-      apply beq_nat_eq in H.
-      congruence.
-    + inversion H.
-    + inversion H.
+    destruct t2; [ auto using beq_nat_eq | inversion H .. ].
   - intros.
-    simpl in H.
     destruct t2.
     + inversion H.
-    + apply andb_true_iff in H.
+    + apply andb_true_iff in H. 
       destruct H.
       apply IHt1_1 in H.
-      apply IHt1_2 in H0.
+      apply IHt1_2 in H0. 
       congruence.
     + inversion H.
   - intros.
-    simpl in H.
     destruct t2.
     + inversion H.
     + inversion H.
@@ -48,148 +40,82 @@ Lemma beq_typ_refl : forall t : typ, beq_typ t t = true.
   - apply andb_true_iff. split. symmetry. apply beq_nat_refl. apply IHt.
 Qed.
 
-Theorem leq_prop : forall m n : nat, true = leq m n <-> m <= n.
+Theorem leq_correct : forall m n : nat, leq m n = true -> m <= n.
   induction m.
-  - intro. simpl. split. intro. auto with arith. tauto.
-  - intro. split.
-    + intro. destruct n.
-      * simpl in H. inversion H.
-      * apply (IHm n) in H. auto with arith.
-    + intro. destruct n. exfalso. apply (le_Sn_0 m). apply H. assert (m <= n). omega. apply IHm. apply H0.
+  - auto with arith.
+  - intros. destruct n.
+    + inversion H.
+    + auto with arith.
 Qed.
 
 (* This is actually cumulativity *)
-Lemma kinding_sub : forall e : env, forall t : typ, forall k k' : kind,
-                       kinding e t k -> k <= k' -> kinding e t k'.
-  intro e0. intro t. generalize e0 as e. clear e0. (* This is ugly *)
-  induction t.
+Lemma kinding_ind_sub : forall (e : env) (t : typ) (k : kind),
+                          kinding_ind e t k -> forall k', k <= k' -> kinding_ind e t k'.
+  do 4 intro.
+  induction H.
   - intros.
-      simpl.
-      simpl in H.
-      remember (get_kind e n) as k1 in H |- *.
-      destruct k1.
-      + split. apply H. destruct H. omega.
-      + apply H.
+    assert (p <= k') by omega.
+    eauto using k_tvar.
   - intros.
-    simpl in H.
-    do 3 destruct H. destruct H1.
-    simpl.
-    exists k'. exists k'.
-    split. auto with arith. split.
-    apply (IHt1 e x). trivial. assert (x <= max x x0). auto with arith. omega.
-    apply (IHt2 e x0). trivial. assert (x0 <= max x x0). auto with arith. omega.
+    destruct k'.
+    + inversion H0.
+    + assert (max p q <= k') by omega.
+      assert (max k' q = k') by eauto with arith.
+      rewrite <- H2.
+      eauto using k_tall with arith.
   - intros.
-    simpl.
-    do 2 destruct H.
-    exists (k' - k0 + (max x k)). split.
-    apply (IHt (etvar k e) x). apply H.
-    assert (x <= max x k). auto with arith. omega.
-    assert (max x k >= k). auto with arith. assert (k' - k0 + max x k >= k). omega.
-    assert (max (k' - k0 + max x k) k = (k' - k0+ max x k)). auto with arith. rewrite H4.
-    rewrite -> H1. assert (S (k' - S (max x k) + max x k) = k' - S (max x k) + S (max x k)).
-    rewrite (plus_comm (k' - S (max x k)) (S (max x k))). rewrite le_plus_minus_r. omega.
-    omega.
-    rewrite -> H5. rewrite (plus_comm). rewrite le_plus_minus_r. trivial.
-    rewrite <- H1. apply H0.
+    assert (p <= max p q /\ q <= max p q) by auto with arith.
+    assert (max k' k' = k') by auto with arith.
+    rewrite <- H3.
+    destruct H2.
+    apply k_tarr; [ eauto using le_trans .. ]. (* TODO just eauto using k_tarr, le_trans doesn't work *)
 Qed.
-      
-Lemma bwf_typ_correct : forall t : typ, forall e : env, bwf_typ e t = true <-> wf_typ e t.
+
+
+(* TODO simplified the equivalences to implications so this plays nice with eauto *)
+Lemma bwf_typ_correct : forall t : typ, forall e : env, bwf_typ e t = true -> wf_typ e t.
   induction t.
-  - intro.
-    simpl.
-    remember (get_kind e n) as k in *.
-    destruct k.
-    + tauto.
-    + split.
-      * intro. discriminate H.
-      * tauto.
-  - intro.
+  - intro. simpl.
+    destruct (get_kind e n); [ intuition .. ].
+  - intros.
+    (* TODO this looks like it could be shorter, but eauto doesn't work *)
+    apply andb_true_iff in H.
     split.
-    + intro.
-      apply andb_true_iff in H.
-      split.
-      * apply IHt1. apply H.
-      * apply IHt2. apply H.
-    + intro.
-      apply andb_true_iff.
-      split.
-      * apply IHt1. apply H.
-      * apply IHt2. apply H.
+    * apply IHt1. apply H.
+    * apply IHt2. apply H.
   - intro. apply IHt.
 Qed.
     
-Lemma bwf_env_correct : forall e : env, bwf_env e = true <-> wf_env e.
+Lemma bwf_env_correct : forall e : env, bwf_env e = true -> wf_env e.
   induction e.
   - simpl. tauto.
-  - split.
-    + intro.
-      apply andb_true_iff in H.
-      split.
-      * apply bwf_typ_correct. apply H.
-      * apply IHe. apply H.
-    + intro.
-      apply andb_true_iff.
-      split.
-      * apply bwf_typ_correct. apply H.
-      * apply IHe. apply H.
-  - split; [ apply IHe; apply H .. ].
+  - intro.
+    apply andb_true_iff in H.
+    split.
+    * apply bwf_typ_correct. apply H.
+    * apply IHe. apply H.
+  - apply IHe.
 Qed.
 
-Theorem kind_of_correct : forall t : typ, forall e : env,
-                            match kind_of e t with
-                              | Some k => kinding e t k
-                              | None => forall k : kind, kinding e t k -> False
-                            end.
+Theorem kind_of_correct (t : typ) : forall (e : env) (k : kind), kind_of e t = Some k -> kinding_ind e t k.
   induction t.
-  - intro.
-    simpl.
-    remember (bwf_env e) as wfe.
-    destruct wfe.
-    + remember (get_kind e n) as k.
-      destruct k.
-      * split.
-        { apply bwf_env_correct. auto. }
-        { auto. }
-      * tauto.
-    + intro. destruct (get_kind e n).
-      * intro.
-        destruct H.
-        apply bwf_env_correct in H.
-        apply (eq_trans Heqwfe) in H.
-        discriminate H.
-      * tauto.
-  - intro.
-    simpl.
-    specialize (IHt1 e).
-    specialize (IHt2 e).
-    remember (kind_of e t1) as k in IHt1 |- * .
-    destruct k.
-    + remember (kind_of e t2) as k2 in IHt2 |- * .
-      destruct k2.
-      * exists k.
-        exists k0.
-        split; [ auto .. ].
-      * intros.
-        do 2 destruct H.
-        apply IHt2 with x0.
-        apply H.
-    + intros.
-      do 2 destruct H.
-      apply IHt1 with x.
-      apply H.
-  - intro.
-    simpl.
-    specialize (IHt (etvar k e)).
-    remember (kind_of (etvar k e) t) as k' in IHt |- *.
-    destruct k'.
-    + exists k0.
-      split. apply IHt. rewrite -> max_comm. trivial.
-    + intros.
-      destruct H.
-      apply IHt with (k0 := x).
-      apply H.
-Qed.
+  - intros. simpl in H.
+    remember (bwf_env e).
+    destruct b.
+    + apply eq_sym in Heqb. eauto using bwf_env_correct, k_tvar.
+    + discriminate H.
+  - intros. simpl in H.
+    remember (kind_of e t1) as kind_of_t1.
+    remember (kind_of e t2) as kind_of_t2.
+    destruct kind_of_t1, kind_of_t2;
+      [ inversion H; eauto using k_tarr | inversion H .. ].
+  - intros. simpl in H.
+    destruct (kind_of (etvar k e) t) eqn:kind_of_etvar.
+    + inversion H. eauto using k_tall.
+    + inversion H.
+Qed. 
 
+(*
 Lemma typing_uniq :
   forall t : term, forall e : env, forall ty1 ty2 : typ,
     typing e t ty1 -> typing e t ty2 -> ty1 = ty2.
@@ -246,7 +172,7 @@ Lemma typing_uniq :
      rewrite H3. rewrite H4.
      congruence.
      apply H0.
-Qed.
+Qed. 
 
 Lemma kind_of_minimal : forall t : typ, forall e : env, forall k : kind,
                           match kind_of e t with
@@ -290,137 +216,44 @@ Lemma kind_of_minimal : forall t : typ, forall e : env, forall k : kind,
       assert (x <= max x k). apply le_max_l.
       omega.
     + trivial.
-Qed.
+Qed. *)
           
-Theorem type_of_correct : forall t : term, forall e : env,
-                            match type_of e t with
-                              | Some ty => typing e t ty
-                              | None => forall ty : typ, typing e t ty -> False
-                            end.
+Theorem type_of_correct (t : term) : forall (e : env) (T : typ), type_of e t = Some T -> typing_ind e t T.
   induction t.
-  - intro. simpl.
-    remember (bwf_env e) as env_bwf.
-    + destruct env_bwf.
-      * remember (get_typ e n) as t.
-        destruct t.
-        { split. apply bwf_env_correct. auto. auto. }
-        { tauto. }
-      * intro.
-        destruct (get_typ e n).
-        { intro. destruct H. apply bwf_env_correct in H. apply (eq_trans Heqenv_bwf) in H. inversion H. }
-        { tauto. }
-  - intro. simpl.
-    specialize (IHt (evar t e)).
-    remember (type_of (evar t e) t0) as ty in IHt |- *.
-    destruct ty.
-    + split. auto. apply IHt.
-    + destruct ty.
-      * auto.
-      * intro.
-        destruct H.
-        rewrite -> H in H0.
-        apply IHt in H0.
-        apply H0.
-      * tauto.
-  - intro.
-    specialize (IHt1 e).
-    specialize (IHt2 e).
-    simpl.
-    remember (type_of e t1) as ty1 in IHt1 |- *.
-    remember (type_of e t2) as ty2 in IHt2 |- *.
-    destruct ty1.
-    + destruct ty2.
-      * destruct t.
-        { intros. do 2 destruct H.
-          apply (typing_uniq t1 e (tvar n) (tarr x ty)) in H.
-          discriminate H.
-          apply IHt1. }
-        { remember (beq_typ t3 t0) as beqt in *.
-          destruct beqt.
-          { exists t3. split.
-            apply IHt1.
-            apply eq_sym in Heqbeqt. apply beq_typ_correct in Heqbeqt.
-            rewrite -> Heqbeqt. apply IHt2.
-          }
-          { intros. do 2 destruct H.
-            apply (typing_uniq t2 e t0 x) in IHt2.
-            apply (typing_uniq t1 e (tarr t3 t4) (tarr x ty)) in IHt1.
-            inversion IHt1.
-            apply eq_sym in IHt2. apply (eq_trans H2) in IHt2.
-            rewrite <- IHt2 in Heqbeqt. 
-            pose proof beq_typ_refl as EqRefl.
-            specialize (EqRefl t3).
-            apply (eq_trans Heqbeqt) in EqRefl. inversion EqRefl.
-            apply H.
-            apply H0.
-          }
-        }
-        { intros. do 2 destruct H.
-          apply (typing_uniq t1 e (tall k t) (tarr x ty)) in IHt1.
-          inversion IHt1.
-          apply H.
-        }
-      * destruct t ; [ intros; destruct H; apply (IHt2 x); apply H .. ].
-    + intros.
-      destruct H.
-      apply (IHt1 (tarr x ty)).
-      apply H.
-  - intros.
-    simpl.
-    remember (type_of (etvar k e) t) as ty1.
-    specialize (IHt (etvar k e)).
-    destruct ty1.
-    + split.
-      * auto.
-      * rewrite <- Heqty1 in IHt.
-        apply IHt.
-    + rewrite <- Heqty1 in IHt.
-      intro.
-      destruct ty.
-      * auto.
-      * auto.
-      * intro. apply (IHt ty). apply H.
-  - intros.
-    simpl.   
-    specialize (IHt e).
-    remember (type_of e t) as ty in IHt |- *.
-    destruct ty.
-    destruct t1.
-    + intros. do 2 destruct H.
-      apply (typing_uniq t e (tvar n) (tall x x0)) in IHt.
-      inversion IHt.
-      apply H.
-    + intros. do 2 destruct H. 
-      apply (typing_uniq t e (tarr t1_1 t1_2) (tall x x0)) in IHt.
-      inversion IHt.
-      apply H.
-    + remember (kind_of e t0) as k0 in *.
-      destruct k0.
-      remember (leq k0 k) as lk0.
-      destruct lk0.
-      * exists k, t1. split. apply IHt. split.
-        pose proof (kind_of_correct t0 e).
-        rewrite <- Heqk0 in H.
-        apply (kinding_sub e t0 k0 k).
-        apply H.
-        apply leq_prop.
-        apply Heqlk0.
-        trivial.
-      * intros.
-        do 3 destruct H. destruct H0.
-        pose proof kind_of_minimal.
-        specialize (H2 t0 e x).
-        rewrite <- Heqk0 in H2.
-        apply H2 in H0.
-        pose proof (typing_uniq t e (tall k t1) (tall x x0) IHt H).
-        inversion H3.
-        pose proof (leq_prop k0 k).
-        destruct H4.
-        rewrite <- H5 in H0. apply H7 in H0. apply eq_sym in H0. apply (eq_trans Heqlk0) in H0.
-        discriminate H0.
-      * intros.
-        do 3 destruct H. destruct H0.
-        pose proof (kind_of_correct t0 e).
-        rewrite <- Heqk0 in H2. apply H2 in H0. apply H0.
-    + intros. do 3 destruct H. apply (IHt (tall x x0)). apply H.
+  - intros. simpl in H.
+    destruct (bwf_env e) eqn:env_is_bwf.
+    + auto using t_var, bwf_env_correct.
+    + inversion H.
+  - intros. simpl in H.
+    destruct (type_of (evar t e) t0) eqn:type_of_body.
+    + inversion H. auto using t_abs.
+    + inversion H.
+  - intros. simpl in H.
+    destruct (type_of e t1) eqn:type_of_fn.
+    + destruct t.
+      * inversion H.
+      * destruct (type_of e t2) eqn:type_of_arg.
+        { destruct (beq_typ t3 t) eqn:equal_types.
+          { inversion H. rewrite <- H1.
+            eauto. apply beq_typ_correct in equal_types. eapply t_app. eauto. rewrite equal_types. eauto. }
+          { inversion H. } }
+        { inversion H. }
+      * inversion H.
+    + inversion H.
+  - intros. simpl in H.
+    destruct (type_of (etvar k e) t) eqn:type_of_body.
+    + inversion H. auto using t_abs_t.
+    + inversion H.
+  - intros. simpl in H.
+    destruct (type_of e t) eqn:?.
+    + destruct t1 eqn:type_of_term.
+      * inversion H.
+      * inversion H.
+      * destruct (kind_of e t0) eqn:kind_of_arg.
+        { destruct (leq k0 k) eqn:k0_leq_k.
+          { inversion H. eapply t_app_t. eauto.
+            eauto using kind_of_correct, leq_correct, kinding_ind_sub, t_app_t. }
+          { inversion H. } }
+        { inversion H. }
+    + inversion H.
 Qed.
